Some new terms and types

Capless/Term.lean
@@ -63,6 +63,12 @@ inductive Term : Nat -> Nat -> Nat -> Type where
 | bindc : CaptureSet n k -> Term n m (k+1) -> Term n m k
 /-- Boundary form `boundary[c] as <c,x> in t`. -/
 | boundary : Classifier -> SType n m k -> Term (n+1) m (k+1) -> Term n m k
+/-- Intercept: `intercept[K] in t` --/
+| intercept : Kind -> Term n m k -> Term n m k
+/-- Unwraps a maybe. --/
+| unwrap : Fin n -> Term n m k
+/-- Unwraps a maybe, but with an additional handler for intercepted labels. --/
+| unwrap_handle : Fin n -> Term (n+2) (m+1) k -> Term n m k
 
 /-!
 ## Notations
@@ -76,6 +82,8 @@ notation:40 "let" "(c,x)=" t " in " u => Term.letex t u
 notation:40 "let" "X=" S " in " t => Term.bindt S t
 notation:40 "let" "c=" C " in " t => Term.bindc C t
 notation:40 "boundary[" c "]:" S " in " t => Term.boundary c S t
+notation:40 "intercept[" K "]"" in " t => Term.intercept K t
+notation:40 "handle " n " with " t => Term.unwrap_handle n t
 
 /-- Whether this term is a value? -/
 @[aesop safe constructors]
@@ -106,6 +114,9 @@ def Term.rename (t : Term n m k) (f : FinFun n n') : Term n' m k :=
   | Term.bindt S t => Term.bindt (S.rename f) (t.rename f)
   | Term.bindc c t => Term.bindc (c.rename f) (t.rename f)
   | Term.boundary c S t => Term.boundary c (S.rename f) (t.rename f.ext)
+  | Term.intercept K t => Term.intercept K (t.rename f)
+  | Term.unwrap x => Term.unwrap (f x)
+  | Term.unwrap_handle x t => Term.unwrap_handle (f x) (t.rename f.ext.ext)
 
 def Term.trename (t : Term n m k) (f : FinFun m m') : Term n m' k :=
   match t with
@@ -123,6 +134,9 @@ def Term.trename (t : Term n m k) (f : FinFun m m') : Term n m' k :=
   | Term.bindt S t => Term.bindt (S.trename f) (t.trename f.ext)
   | Term.bindc c t => Term.bindc c (t.trename f)
   | Term.boundary c S t => Term.boundary c (S.trename f) (t.trename f)
+  | Term.intercept K t => Term.intercept K (t.trename f)
+  | Term.unwrap x => Term.unwrap x
+  | Term.unwrap_handle x t => Term.unwrap_handle x (t.trename f.ext)
 
 def Term.crename (t : Term n m k) (f : FinFun k k') : Term n m k' :=
   match t with
@@ -140,6 +154,9 @@ def Term.crename (t : Term n m k) (f : FinFun k k') : Term n m k' :=
   | Term.bindt S t => Term.bindt (S.crename f) (t.crename f)
   | Term.bindc c t => Term.bindc (c.crename f) (t.crename f.ext)
   | Term.boundary c S t => Term.boundary c (S.crename f) (t.crename f.ext)
+  | Term.intercept K t => Term.intercept K (t.crename f)
+  | Term.unwrap x => Term.unwrap x
+  | Term.unwrap_handle x t => Term.unwrap_handle x (t.crename f)
 
 def Term.weaken (t : Term n m k) : Term (n+1) m k := t.rename FinFun.weaken
 
@@ -248,6 +265,12 @@ theorem Term.rename_id {t : Term n m k} :
     simp [Term.rename, CaptureSet.rename_id, ih]
   case boundary ih =>
     simp [Term.rename, SType.rename_id, ih, FinFun.id_ext]
+  case intercept ih =>
+    simp [Term.rename, ih]
+  case unwrap =>
+    simp [Term.rename, FinFun.id]
+  case unwrap_handle ih =>
+    simp [Term.rename, FinFun.id_ext, ih, FinFun.id]
 
 theorem Term.trename_id {t : Term n m k} :
   t.trename FinFun.id = t := by
@@ -285,6 +308,12 @@ theorem Term.trename_id {t : Term n m k} :
     exact ih
   case boundary ih =>
     simp [Term.trename, SType.trename_id, ih, FinFun.id_ext]
+  case intercept ih =>
+    simp [Term.trename, ih]
+  case unwrap =>
+    simp [Term.trename]
+  case unwrap_handle ih =>
+    simp [Term.trename, FinFun.id_ext, ih]
 
 theorem Term.crename_id {t : Term n m k} :
   t.crename FinFun.id = t := by
@@ -322,6 +351,12 @@ theorem Term.crename_id {t : Term n m k} :
   case boundary ih =>
     simp [Term.crename]
     simp [ih, SType.crename_id, FinFun.id_ext]
+  case intercept ih =>
+    simp [Term.crename, ih]
+  case unwrap =>
+    simp [Term.crename]
+  case unwrap_handle ih =>
+    simp [Term.crename, ih]
 
 theorem Term.rename_rename {t : Term n m k} {f : FinFun n n'} {g : FinFun n' n''} :
   (t.rename f).rename g = t.rename (g.comp f) := by
@@ -360,6 +395,13 @@ theorem Term.rename_rename {t : Term n m k} {f : FinFun n n'} {g : FinFun n' n''
     simp [<- FinFun.ext_comp_ext, ih]
   case boundary ih =>
     simp [rename, SType.rename_rename]
+    simp [<- FinFun.ext_comp_ext, ih]
+  case intercept ih =>
+    simp [rename, ih]
+  case unwrap =>
+    simp [rename]
+  case unwrap_handle ih =>
+    simp [rename]
     simp [<- FinFun.ext_comp_ext, ih]
 
 theorem Term.crename_crename {t : Term n m k} {f : FinFun k k'} {g : FinFun k' k''} :
@@ -400,6 +442,12 @@ theorem Term.crename_crename {t : Term n m k} {f : FinFun k k'} {g : FinFun k' k
   case boundary ih =>
     simp [crename, SType.crename_crename]
     simp [<- FinFun.ext_comp_ext, ih]
+  case intercept ih =>
+    simp [crename, ih]
+  case unwrap =>
+    simp [crename]
+  case unwrap_handle ih =>
+    simp [crename, ih]
 
 theorem Term.trename_trename {t : Term n m k} {f : FinFun m m'} {g : FinFun m' m''} :
   (t.trename f).trename g = t.trename (g.comp f) := by
@@ -438,6 +486,13 @@ theorem Term.trename_trename {t : Term n m k} {f : FinFun m m'} {g : FinFun m' m
     simp [<- FinFun.ext_comp_ext, ih]
   case boundary ih =>
     simp [trename, SType.trename_trename]
+    simp [<- FinFun.ext_comp_ext, ih]
+  case intercept ih =>
+    simp [trename, ih]
+  case unwrap =>
+    simp [trename]
+  case unwrap_handle ih =>
+    simp [trename]
     simp [<- FinFun.ext_comp_ext, ih]
 
 end Capless
