Capless/Type/Basic.lean
@@ -83,6 +83,9 @@ theorem SType.crename_rename_comm (S : SType n m k) (f : FinFun n n') (g : FinFu
   | SType.label S => by
     have ih := SType.crename_rename_comm S f g
     simp [SType.rename, SType.crename, ih]
+  | SType.maybe T => by
+    have ih := SType.crename_rename_comm T f g
+    simp [SType.rename, SType.crename, ih]
 
 end
 
@@ -148,6 +151,9 @@ theorem SType.rename_rename (S : SType n m k) (f : FinFun n n') (g : FinFun n' n
   | SType.label S => by
     have ih := SType.rename_rename S f g
     simp [SType.rename, ih]
+  | SType.maybe T => by
+    have ih := SType.rename_rename T f g
+    simp [SType.rename, ih]
 
 end
 
@@ -205,6 +211,9 @@ theorem SType.trename_rename_comm (S : SType n m k) (f : FinFun n n') (g : FinFu
   | SType.label S => by
     have ih := SType.trename_rename_comm S f g
     simp [SType.trename, SType.rename, ih]
+  | SType.maybe T => by
+    have ih := SType.trename_rename_comm T f g
+    simp [SType.trename, SType.rename, ih]
 
 end
 
@@ -249,6 +258,9 @@ theorem SType.crename_crename (S : SType n m k) (f : FinFun k k') (g : FinFun k'
   | SType.label S => by
     have ih := SType.crename_crename S f g
     simp [SType.crename, ih]
+  | SType.maybe T => by
+    have ih := SType.crename_crename T f g
+    simp [SType.crename, ih]
 
 end
 
@@ -292,6 +304,9 @@ theorem SType.crename_trename_comm (S : SType n m k) (f : FinFun k k') (g : FinF
     simp [SType.crename, SType.trename, ih]
   | SType.label S => by
     have ih := SType.crename_trename_comm S f g
+    simp [SType.crename, SType.trename, ih]
+  | SType.maybe T => by
+    have ih := SType.crename_trename_comm T f g
     simp [SType.crename, SType.trename, ih]
 
 end
@@ -425,6 +440,9 @@ theorem SType.trename_trename (S : SType n m k) (f : FinFun m m') (g : FinFun m'
   | SType.label S => by
     have ih := SType.trename_trename S f g
     simp [SType.trename, ih]
+  | SType.maybe T => by
+    have ih := SType.trename_trename T f g
+    simp [SType.trename, ih]
 
 end
 
@@ -544,6 +562,9 @@ theorem SType.rename_id {S : SType n m k} :
   | SType.label S => by
     have ih := SType.rename_id (S := S)
     simp [SType.rename, ih]
+  | SType.maybe T => by
+    have ih := SType.rename_id (S := T)
+    simp [SType.rename, ih]
 
 end
 
@@ -587,6 +608,9 @@ theorem SType.trename_id {S : SType n m k} :
     simp [SType.trename, ih]
   | SType.label S => by
     have ih := SType.trename_id (S := S)
+    simp [SType.trename, ih]
+  | SType.maybe T => by
+    have ih := SType.trename_id (S := T)
     simp [SType.trename, ih]
 
 end
@@ -632,6 +656,9 @@ theorem SType.crename_id {S : SType n m k} :
     simp [SType.crename, ih]
   | SType.label S => by
     have ih := SType.crename_id (S := S)
+    simp [SType.crename, ih]
+  | SType.maybe T => by
+    have ih := SType.crename_id (S := T)
     simp [SType.crename, ih]
 
 end
